\documentclass[12pt]{article}
\usepackage[paper=letterpaper,margin=2cm]{geometry}
\usepackage{amsmath}
\usepackage{amssymb}
\usepackage{amsfonts}
\usepackage{newtxtext, newtxmath}
\usepackage{enumitem}
\usepackage{titling}
\usepackage[colorlinks=true]{hyperref}

\setlength{\droptitle}{-6em}

% Enter the specific assignment number and topic of that assignment below, and replace "Your Name" with your actual name.
\title{An extension to t hints}
\author{Rui Tang}
\date{\today}

\begin{document}
\maketitle

Suppose there are t hints invloved, namely
$$
H=
\begin{bmatrix}
R&0 \\
0&R
\end{bmatrix}
\begin{bmatrix}
A_{1}^1&A_{1}^2&\dots&A_{1}^t \\
A_{2}^1&A_{2}^2&\dots&A_{2}^t
\end{bmatrix}
\begin{bmatrix}
R^{-1} &  &  \\  
  & \ddots  &  \\
 &  & R^{-1}
\end{bmatrix},
$$

where $RR^{T}=nI_n$, $R^{-1}(R^T)^{-1}=\frac{1}{n}I_n$, and $R$ is an orthogonal matrix scaled by $\sqrt{n}$. Then,

\begin{align*}
\quad&\det \left( H^{T}\Sigma H+\Sigma_{\epsilon} \right)\\
=&\det\left( I_{2n}+\frac{1}{\sigma_{\epsilon}^2}\Sigma^{1/2}HH^T\Sigma^{1/2} \right)\det(\Sigma_{\epsilon})\\
=&\det\left( I_{2n}+\frac{1}{\sigma_{\epsilon}^2}
\begin{bmatrix}
R\left( \frac{1}{n}\sigma_{s}^2\sum_{j=1}^t A_{1}^j(A_{1}^{j})^T \right)R^T & R\left( \frac{1}{n}\sigma_{s}\sigma_{e}\sum_{j=1}^t A_{1}^j(A_{2}^{j})^T \right)R^T \\
R\left( \frac{1}{n}\sigma_{s}\sigma_{e}\sum_{j=1}^t A_{2}^j(A_{1}^{j})^T \right)R^T & R\left( \frac{1}{n}\sigma_{e}^2\sum_{j=1}^t A_{2}^j(A_{2}^{j})^T \right)R^T
\end{bmatrix}
\right)\det(\Sigma_{\epsilon})\\
=&\det \left( 
\begin{bmatrix}
\frac{\sigma_{s}^2}{\sigma_{\epsilon}^2}\sum_{j=1}^t A_{1}^j(A_{1}^{j})^T+I_{n}  & \frac{\sigma_{s}\sigma_{e}}{\sigma_{\epsilon}^2}\sum_{j=1}^t A_{1}^j(A_{2}^{j})^T  \\
 \frac{\sigma_{s}\sigma_{e}}{\sigma_{\epsilon}^2}\sum_{j=1}^t A_{2}^j(A_{1}^{j})^T  &  \frac{\sigma_{e}^2}{\sigma_{\epsilon}^2}\sum_{j=1}^t A_{2}^j(A_{2}^{j})^T+I_{n} 
\end{bmatrix}
\right)\det(\Sigma_{\epsilon})\\
\stackrel{(a)}{=}&\det
\begin{bmatrix}
S_{1} & 0 & \dots & 0 &  0 \\
0 & S_{2} & \dots & 0 & 0 \\
\vdots & \vdots & \ddots & \vdots & \vdots \\
0 & 0 & \dots & S_{\frac{n}{2}-1} & 0 \\
0 & 0 & \dots & 0 & S_{\frac{n}{2}}
\end{bmatrix}\det(\Sigma_{\epsilon})\\
=&\det(\Sigma_{\epsilon})\prod_{i=1}^{n/2}\det(S_{i})\\
=&\sigma_\epsilon^{2tn}\prod_{i=1}^{n/2}
\frac{\sigma_{s}^4\sigma_{e}^4}{16\sigma_{\epsilon}^{8}}
\Bigg( 
\left( \sum_{j=1}^t\left( (V_{i,h_{s}}^{j})^2+(V_{n-i,h_{s}}^{j})^2\right)+\frac{2\sigma^2_\epsilon}{\sigma_s^2} \right) \left( \sum_{j=1}^t\left( (V_{i,h_{e}}^{j})^2+(V_{n-i,h_{e}}^{j})^2\right)+\frac{2\sigma^2_\epsilon}{\sigma_e^2} \right) \\
\quad&-
\left( \sum_{j=1}^t\left( V_{i,h_{s}}^{j}V_{i,h_{e}}^j+V_{n-i,h_{s}}^{j}V_{n-i,h_{e}}^j\right) \right)^2 
-
\left( \sum_{j=1}^t\left( V_{i,h_{s}}^{j}V_{n-i,h_{e}}^j-V_{i,h_{e}}^{j}V_{n-i,h_{s}}^j\right) \right) ^2
\Bigg) ^2\\
=&\left(\frac{\sigma^4_s\sigma^4_e}{16\sigma^{8-4t}_\epsilon}\right)^{\frac{n}{2}}\prod_{i=1}^{\frac{n}{2}}\Bigg(
\sum_{1\leq j\neq k \leq t}\Bigg(
\left(V_{i,h_s}^j V_{i,h_e}^k \right)^2 +
\left(V_{i,h_s}^j V_{n-i,h_e}^k \right)^2 +
\left(V_{n-i,h_s}^j V_{i,h_e}^k \right)^2 +
\left(V_{n-i,h_s}^j V_{n-i,h_e}^k \right)^2 \\
\quad&-
\left( V_{i,h_s}^j V_{i,h_e}^j V_{i,h_s}^k V_{i,h_e}^k +
V_{n-i,h_s}^j V_{n-i,h_e}^j V_{n-i,h_s}^k V_{n-i,h_e}^k +
V_{i,h_s}^j V_{n-i,h_e}^j V_{i,h_s}^k V_{n-i,h_e}^k +
V_{n-i,h_s}^j V_{i,h_e}^j V_{n-i,h_s}^k V_{n-i,h_e}^k
\right)
\Bigg)\\
\quad&+\frac{2\sigma_\epsilon^2}{\sigma_s^2} \sum_{j=1}^t 
\left(
\left( (V_{i,h_e}^j \right)^2 +
\left( (V_{n-i,h_e}^j \right)^2
\right)
+\frac{2\sigma_\epsilon^2}{\sigma_e^2} \sum_{j=1}^t 
\left(
\left( (V_{i,h_s}^j \right)^2 +
\left( (V_{n-i,h_s}^j \right)^2 
\right)
+4\frac{\sigma_\epsilon^4}{\sigma_s^2\sigma_e^2}
\Bigg)^2,
\end{align*}

where
$$
\det S_{i}
=\det
\begin{bmatrix}
a_{i} & 0 & c_{i} & -d_{i} \\
0 & a_{i} & d_{i} & c_{i} \\
c_{i} & d_{i} & b_{i} & 0 \\
-d_{i} & c_{i} & 0 & b_{i}
\end{bmatrix}
=\det
\begin{bmatrix}
A & B \\
C & D 
\end{bmatrix}
=\det
(AD-BC),
$$
$$
\det
(AD-BC)
=\det
\left( 
\begin{bmatrix}
a_{i}b_{i} & 0 \\
0 & a_{i}b_{i} 
\end{bmatrix}-
\begin{bmatrix}
c_{i} & -d_{i} \\
d_{i} & c_{i}
\end{bmatrix}
\begin{bmatrix}
c_{i} & d_{i} \\
-d_{i} & c_{i}
\end{bmatrix}
\right) 
=(a_{i}b_{i}-c_{i}^2-d_{i}^2)^2,
$$
$$
a_{i}=\frac{\sigma_{s}^2}{2\sigma_{\epsilon}^2}\sum_{j=1}^t\left( (V_{i,h_{s}}^{j})^2+(V_{n-i,h_{s}}^{j})^2+\frac{2\sigma_\epsilon^2}{\sigma_s^2}\right),
$$
$$
b_{i}=\frac{\sigma_{e}^2}{2\sigma_{\epsilon}^2}\sum_{j=1}^t\left( (V_{i,h_{e}}^{j})^2+(V_{n-i,h_{e}}^{j})^2+\frac{2\sigma_\epsilon^2}{\sigma_e^2}\right),
$$
$$
c_{i}=\frac{\sigma_{s}\sigma_{e}}{2\sigma_{\epsilon}^2}\sum_{j=1}^t\left( V_{i,h_{s}}^{j}V_{i,h_{e}}^j+V_{n-i,h_{s}}^{j}V_{n-i,h_{e}}^j\right),
$$
$$
d_{i}=\frac{\sigma_{s}\sigma_{e}}{2\sigma_{\epsilon}^2}\sum_{j=1}^t\left( V_{i,h_{s}}^{j}V_{n-i,h_{e}}^j-V_{i,h_{e}}^{j}V_{n-i,h_{s}}^j\right).
$$



Identify
\begin{align*}
    Y_i:=&\,\sum_{1\leq j\neq k \leq t}\Bigg(
\left(V_{i,h_s}^j V_{i,h_e}^k \right)^2 +
\left(V_{i,h_s}^j V_{n-i,h_e}^k \right)^2 +
\left(V_{n-i,h_s}^j V_{i,h_e}^k \right)^2 +
\left(V_{n-i,h_s}^j V_{n-i,h_e}^k \right)^2 \\
-&
\left( V_{i,h_s}^j V_{i,h_e}^j V_{i,h_s}^k V_{i,h_e}^k +
V_{n-i,h_s}^j V_{n-i,h_e}^j V_{n-i,h_s}^k V_{n-i,h_e}^k +
V_{i,h_s}^j V_{n-i,h_e}^j V_{i,h_s}^k V_{n-i,h_e}^k +
V_{n-i,h_s}^j V_{i,h_e}^j V_{n-i,h_s}^k V_{n-i,h_e}^k
\right)
\Bigg)\\
\quad&+\frac{2\sigma_\epsilon^2}{\sigma_s^2} \sum_{j=1}^t 
\left(
\left( (V_{i,h_e}^j \right)^2 +
\left( (V_{n-i,h_e}^j \right)^2
\right)
+\frac{2\sigma_\epsilon^2}{\sigma_e^2} \sum_{j=1}^t 
\left(
\left( (V_{i,h_s}^j \right)^2 +
\left( (V_{n-i,h_s}^j \right)^2 
\right)
+4\frac{\sigma_\epsilon^4}{\sigma_s^2\sigma_e^2}.
\end{align*}

Since  $\{V_{i,h_s}^j\}_{j=1;i=1}^{t;n}$ and $\{V_{i,h_e}^j\}_{j=1;i=1}^{t;n}$ are mutually independent, the expectation of the product is the product of each expectation,
$$\mathbb{E}\det \left( H^{T}\Sigma H+\Sigma_{\epsilon}\right)
=\left(\frac{\sigma_s^4\sigma_e^4}{16\sigma_\epsilon^{8-4t}}\right)^{\frac{n}{2}}\prod_{i=1}^{\frac{n}{2}}\mathbb{E}Y^2
=\left(\frac{\sigma_s^4\sigma_e^4}{16\sigma_\epsilon^{8-4t}}\right)^{\frac{n}{2}}\prod_{i=1}^{\frac{n}{2}}\left(\textrm{Var} Y+\mathbb{E}^2Y\right),
$$
where
$$
\textrm{Var} Y=28t(t-1)n^4\sigma_{h_s}^4\sigma_{h_e}^4+16tn^2\sigma_\epsilon^4(\frac{\sigma_{h_s}^4}{\sigma_e^4}+\frac{\sigma_{h_e}^4}{\sigma_s^4}),
$$
$$
\mathbb{E}^2Y=\left(4t(t-1)n^2\sigma_{h_s}^2\sigma_{h_e}^2+4tn\sigma_\epsilon^2(\frac{\sigma_{h_s}^2}{\sigma_e^2}+\frac{\sigma_{h_e}^2}{\sigma_s^2})+4\frac{\sigma_\epsilon^4}{\sigma_s^2\sigma_e^2}
\right)^2.
$$
Then
\begin{align*}
\quad&\mathbb{E}\det \left( H^{T}\Sigma H+\Sigma_{\epsilon}\right)\\
=&\left(\sigma_{s}^4\sigma_{e}^4\sigma_\epsilon^{4t-8}\left(
\frac{7}{4}t(t-1)n^4\sigma_{h_s}^4\sigma_{h_e}^4+tn^2\sigma_\epsilon^{4}(\frac{\sigma_{h_s}^4}{\sigma_e^4}+\frac{\sigma_{h_e}^4}{\sigma_s^4})
+
\left(
t(t-1)n^2\sigma_{h_s}^2\sigma_{h_e}^2+tn\sigma_\epsilon^2(\frac{\sigma_{h_s}^2}{\sigma_e^2}+\frac{\sigma_{h_e}^2}{\sigma_s^2})+\frac{\sigma_{\epsilon}^4}{\sigma_s^2\sigma_e^2}
\right)^2
\right)
\right)^{\frac{n}{2}}.
\end{align*}



\end{document}

